ITP final project

Automata/Collapse.lean
@@ -2,77 +2,10 @@ import Mathlib.Tactic
 import Automata.DFA
 import Automata.Input
 import Automata.Equality
-
-/-
-1. General Equality
-2. The Collapse Problem
-3. Fin operations? Mathlib weird
-4. Casting!
-5. Writeup?
-
--/
-
-variable {α : Type} {n : ℕ} {b : ℕ}
-
--- Auxilliary functions for collapse
-def tail (f: Fin (n+1) → α) : Fin n → α :=
-  fun i => f (i.succ)
-
-#check Fin.insertNth
-
-def remove_index (i : Fin (n + 1)) (f: Fin (n + 1) → α):
-   (Fin n → α) :=
-    fun j => f (if j.val < i.val then j else ⟨j.val + 1, by omega⟩)
-
-def recover_index (i : Fin (n + 1)) (k: Fin n) (f: Fin n → α):
-   (Fin (n + 1) → α) :=
-    fun j => if hlt : j < i then f ⟨j, by omega⟩ else if hgt : j > i then f ⟨j - 1, by omega⟩ else f k
+import Automata.Fin
 
 
-
-theorem remove_recover (i : Fin (n + 1)) (k: Fin n) (f: Fin n → α) :
-  remove_index i (recover_index i k f) = f := by
-  ext x
-  simp[remove_index, recover_index]
-  split; simp only [Fin.coe_castSucc, Fin.eta, dite_eq_ite, ite_eq_then, not_lt]
-  . intro h
-    have : i.val ≤ x.val := by exact h
-    omega
-  . split
-    . rename_i hsucc h
-      have : x.val + 1 < i.val := by
-        simp_all only [not_lt]
-        exact h
-      omega
-    . split
-      . rfl
-      . rename_i h₁ h₂ h₃
-        have : ¬ x.val + 1 < i.val := by
-          simp_all only [not_lt]
-          exact h₂
-        have : ¬ i.val < x.val + 1 := by
-          simp_all only [not_lt]
-          exact h₃
-        omega
-
-theorem recover_remove (i : Fin (n + 1)) (k: Fin n) (f: Fin (n + 1) → α) (hf: f i = f k) (hik : i.val > k.val ) :
-  recover_index i k (remove_index i f) = f := by
-  ext x
-  simp[remove_index, recover_index]
-  split; simp only [Fin.coe_castSucc, Fin.eta, dite_eq_ite, ite_eq_then, not_lt]
-  . split; simp_all
-    . split
-      .
-        -- have : i.val < x.val := by omega
-
-        omega
-      . rcases x with ⟨x, hx⟩
-        cases x; contradiction
-        rfl
-    . simp_all only [Fin.coe_eq_castSucc, gt_iff_lt, not_lt]
-      have : x = i := by omega
-      subst this
-      simp_all only [le_refl]
+variable {α : Type} {n : ℕ}
 
 def collapse (i : Fin (n+1)) (k : Fin n) (dfa : DFA (Fin (n+1) → α) state) : DFA (Fin n → α) state := {
   transition := fun a q => dfa.transition (recover_index i k a) q
@@ -120,12 +53,75 @@ theorem collapse_correct (dfa : DFA (Fin (n + 1) → Fin (b + 2)) state) (l : Li
       . exact List.getElem?_mem h₁
 
   intro v hv
-  dsimp
-  rw[recover_remove]
+  dsimp only [Function.comp_apply]
+  -- rw[recover_remove]
+  rw[recover_index, insert_remove]
+  rw[remove_index, Fin.succAbove, Fin.castSucc, Fin.castAdd, Fin.castLE]
+  split;
   specialize this v hv
   .
-    simp_all only [Fin.getElem_fin, gt_iff_lt, Fin.eta, Fin.coe_eq_castSucc]
+    simp_all only [Fin.getElem_fin, gt_iff_lt, Fin.eta]
     ext : 1
     simp_all only
-    rfl
-  . exact hik
+  . rename_i h
+    have : ¬ k.val < i := by
+      -- AESOP failed
+      apply h
+    simp_all only [Fin.getElem_fin, gt_iff_lt]
+
+
+-- Legacy
+
+-- Auxilliary functions for collapse
+
+-- def remove_index (i : Fin (n + 1)) (f: Fin (n + 1) → α):
+--    (Fin n → α) :=
+--     fun j => f (if j.val < i.val then j else ⟨j.val + 1, by omega⟩)
+
+-- def recover_index (i : Fin (n + 1)) (k: Fin n) (f: Fin n → α):
+--    (Fin (n + 1) → α) :=
+--     fun j => if hlt : j < i then f ⟨j, by omega⟩ else if hgt : j > i then f ⟨j - 1, by omega⟩ else f k
+
+-- theorem remove_recover (i : Fin (n + 1)) (k: Fin n) (f: Fin n → α) :
+--   remove_index i (recover_index i k f) = f := by
+--   ext x
+--   simp[remove_index, recover_index]
+--   split; simp only [Fin.coe_castSucc, Fin.eta, dite_eq_ite, ite_eq_then, not_lt]
+--   . intro h
+--     have : i.val ≤ x.val := by exact h
+--     omega
+--   . split
+--     . rename_i hsucc h
+--       have : x.val + 1 < i.val := by
+--         simp_all only [not_lt]
+--         exact h
+--       omega
+--     . split
+--       . rfl
+--       . rename_i h₁ h₂ h₃
+--         have : ¬ x.val + 1 < i.val := by
+--           simp_all only [not_lt]
+--           exact h₂
+--         have : ¬ i.val < x.val + 1 := by
+--           simp_all only [not_lt]
+--           exact h₃
+--         omega
+
+-- theorem recover_remove (i : Fin (n + 1)) (k: Fin n) (f: Fin (n + 1) → α) (hf: f i = f k) (hik : i.val > k.val ) :
+--   recover_index i k (remove_index i f) = f := by
+--   ext x
+--   simp[remove_index, recover_index]
+--   split; simp only [Fin.coe_castSucc, Fin.eta, dite_eq_ite, ite_eq_then, not_lt]
+--   . split; simp_all
+--     . split
+--       .
+--         -- have : i.val < x.val := by omega
+
+--         omega
+--       . rcases x with ⟨x, hx⟩
+--         cases x; contradiction
+--         rfl
+--     . simp_all only [Fin.coe_eq_castSucc, gt_iff_lt, not_lt]
+--       have : x = i := by omega
+--       subst this
+--       simp_all only [le_refl]
