Automata/Projection.lean
@@ -6,22 +6,9 @@ import Automata.DFA
 import Automata.NFA
 import Automata.Pumping
 import Automata.Input
-import Automata.LeadingZeroes
-
+import Automata.LeadingZeros
+import Automata.Fin
 import Automata.Collapse
-
-
-
--- Auxilliary theorems for recover
-theorem finLt (m : Fin (n+1)) (b : ℕ) : b < m.val → b < n := by omega
-
-theorem finPred (m : Fin n) (a : Fin n) (h : a > m): a.val - 1 < n - 1 := by omega
-
--- Auxilliary function for project
-def recover_value (m : Fin (n + 1)) (x: Fin (b+2)) (f: Fin n → Fin (b+2)) :
- (Fin (n + 1) → Fin (b+2)) :=
-    fun i => if h1: i.val < m.val then f ⟨i.val, finLt m i.val h1⟩
-      else if h2: i.val > m.val then f ⟨i.val - 1, finPred m i h2⟩ else x
 
 def project (m : Fin (n+1)) (dfa : DFA (Fin (n+1) → Fin (b+2)) state) [DecidableEq state] :
   NFA (Fin n → Fin (b+2)) state := {
@@ -32,139 +19,83 @@ def project (m : Fin (n+1)) (dfa : DFA (Fin (n+1) → Fin (b+2)) state) [Decidab
   output := dfa.output
 }
 
-theorem project_accept [DecidableEq state](dfa : DFA (Fin (n + 1) → Fin (b+2)) state) (m : Fin (n + 1)) (l : List (Fin n → Fin (b+2))) : dfa.eval (l.map (recover_value m x)) → (project m dfa).eval l := by
+theorem project_transition [DecidableEq state](dfa : DFA (Fin (n + 1) → Fin (b+2)) state) (m : Fin (n + 1)) (f : (Fin (n+1) → Fin (b+2))) (p q : state) : dfa.transition f p = q → q ∈ ((project m dfa).transition (remove_index m f) p).val := by
+  simp only [project, List.mem_dedup, List.mem_map, FinEnum.mem_toList, true_and]
+  intro h
+  use f m
+  simp[recover_value, insert_remove]
+  exact h
+
+theorem project_transition' [DecidableEq state](dfa : DFA (Fin (n + 1) → Fin (b+2)) state) (m : Fin (n + 1)) (f : (Fin (n+1) → Fin (b+2))) (p : state) : dfa.transition f p ∈ ((project m dfa).transition (remove_index m f) p).val := by
+  simp only [project, List.mem_dedup, List.mem_map, FinEnum.mem_toList, true_and]
+  use f m
+  simp[recover_value, insert_remove]
+
+
+theorem project_transFrom [DecidableEq state](dfa : DFA (Fin (n + 1) → Fin (b+2)) state) (m : Fin (n + 1)) (l : List (Fin (n+1) → Fin (b+2))) (p q : state) : dfa.transFrom l p = q → q ∈ ((project m dfa).transFrom (l.map (fun f => remove_index m f)) ⟨[p], by exact List.nodup_singleton p⟩).val := by
+  intro h
+  induction l generalizing p
+  case nil =>
+    simp_all only [List.map_nil]
+    simp only [DFAO.transFrom] at h
+    simp only [NFA.transFrom, List.mem_singleton]
+    exact h.symm
+  case cons f fs ih =>
+    simp[DFAO.transFrom] at h
+    simp[NFA.transFrom, NFA.transList]
+    specialize ih (dfa.transition f p) h
+    have := NFA.transFrom_sublist (ps := ⟨[dfa.transition f p], by exact List.nodup_singleton (dfa.transition f p)⟩) (project m dfa) (List.map (fun f ↦ remove_index m f) fs) ⟨(((project m dfa).transition (remove_index m f) p).val).dedup, by apply List.nodup_dedup⟩
+    apply this
+    . simp only [List.cons_subset, List.mem_dedup, List.nil_subset, and_true]
+      apply project_transition'
+    . assumption
+
+theorem project_evalFrom [DecidableEq state](dfa : DFA (Fin (n + 1) → Fin (b+2)) state) (m : Fin (n + 1)) (l : List (Fin (n+1) → Fin (b+2))) (p : state) : dfa.evalFrom l p → (project m dfa).evalFrom (l.map (fun f => remove_index m f)) ⟨[p], by exact List.nodup_singleton p⟩ := by
+  simp[NFA.evalFrom, DFAO.evalFrom]
+  intro h
+  use (DFAO.transFrom dfa l p)
+  constructor
+  . apply project_transFrom
+    rfl
+  . simp only [project]
+    exact h
+
+theorem project_eval [DecidableEq state](dfa : DFA (Fin (n + 1) → Fin (b+2)) state) (m : Fin (n + 1)) (l : List (Fin (n+1) → Fin (b+2))) : dfa.eval l → (project m dfa).eval (l.map (fun f => remove_index m f)) := by
+  simp[NFA.eval, DFAO.eval]
+  exact project_evalFrom dfa m l dfa.start
+
+
+theorem project_acceptZero [DecidableEq state] (dfa : DFA (Fin (n + 1) → Fin (b+2)) state) (h: DFA.respectZero dfa) (m : Fin (n + 1)) : NFA.acceptZero (project m dfa) := by
   sorry
 
-theorem project_acceptZero [DecidableEq state] (dfa : DFA (Fin (n + 1) → Fin (b+2)) state) (h: DFA.acceptZero dfa) (m : Fin (n + 1)) : NFA.acceptZero (project m dfa) := by
-  simp only [DFA.acceptZero, NFA.acceptZero] at *
-  intro x hx z
-  simp only [project, NFA.eval, NFA.transFrom, recover_value]
+theorem project_correct [Fintype state] [DecidableEq state] (l : List ℕ) (hl : l.length = len)(m : Fin (len + 1)) (dfa : DFA (Fin (len +1) → Fin (b+2)) state) (h: dfa.acceptZero):
+  ∃ (x : ℕ), dfa.eval (inputToBase (b+2) (by norm_num) (l.insertNth m x) (by simp_rw[← hl]; apply List.length_insertNth; omega)) ↔ (project m dfa).eval (padZeroes (Fintype.card (ListND state)) (inputToBase (b+2) (by omega) l hl)):= by
   sorry
 
-theorem DFAO.bounded_out [Fintype state] (dfao : DFAO (Fin n → Fin (b+2)) state out) (x : List (Fin n → Fin (b+2))) (o: out)(h: ∀ (x : List (Fin n → Fin (b+2))), dfao.eval x = o → (∀ m, dfao.eval (padZeroes m x) = o)) : ∀ k, dfao.eval (padZeroes k x) = o → dfao.eval (padZeroes (Fintype.card state) x) = o := by
-  rintro k hkxo
-  by_cases hkstate : k ≤ Fintype.card state
-  . have: Fintype.card state = (Fintype.card state - k) + k := by omega
-    rw[this, ← padZeroes_add (Fintype.card state - k) k x]
-    apply h
-    exact hkxo
+-- Legacy
 
-  simp only [not_le] at hkstate
-  -- Question: How to get this kind of descent argument work in lean?
-  . induction' hk : k - Fintype.card state using Nat.strong_induction_on  with d ih generalizing k
-    have hkxlen : Fintype.card state ≤ (padZeroes k x).length := by
-      simp only [padZeroes_length]
-      omega
+-- Auxilliary theorems for recover
+-- theorem finLt (m : Fin (n+1)) (b : ℕ) : b < m.val → b < n := by omega
 
-    obtain ⟨a, b', c, hkxabc, hablen, hne, hy⟩ := dfao.pumping_lemma_eval hkxo hkxlen
-    have haco : dfao.eval (a ++ c) = o := by
-      apply hy
-      simp only [Language.mem_mul, exists_exists_and_exists_and_eq_and, List.append_assoc]
-      use a, (by exact rfl), [], (by exact Language.nil_mem_kstar {b'}), c, (by exact rfl)
-      simp only [List.nil_append]
-    -- have hblen : 0 < b'.length := by
-    --   exact List.length_pos_of_ne_nil hne
+-- theorem finPred (m : Fin n) (a : Fin n) (h : a > m): a.val - 1 < n - 1 := by omega
 
-    have habzero : ∀ i, ∀ (hi: i < a.length + b'.length),  (a ++ b')[i]' (by rw[List.length_append]; exact hi) = fun _ => 0 := by
-      intro i hi
-      rw[← List.getElem_append_left (a++b') c]
-      trans (padZeroes k x)[i]
-      congr 1
-      . exact hkxabc.symm
-      . apply padZeroes_zero k
-        omega
-      simp only [List.append_assoc, List.length_append]
-      . omega
+-- -- Auxilliary function for project
+-- def recover_value (m : Fin (n + 1)) (x: Fin (b+2)) (f: Fin n → Fin (b+2)) :
+--  (Fin (n + 1) → Fin (b+2)) :=
+--     fun i => if h1: i.val < m.val then f ⟨i.val, finLt m i.val h1⟩
+--       else if h2: i.val > m.val then f ⟨i.val - 1, finPred m i h2⟩ else x
 
-    have hazero : ∀ i, ∀ (hi: i < a.length),  a[i]' (by omega) = fun _ => 0 := by
-      intro i hi
-      rw[← List.getElem_append_left a b']
-      apply habzero i
-      . omega
-    have hbzero : ∀ i, ∀ (hi: i < b'.length),  b'[i]' (by omega) = fun _ => 0 := by
-      intro i hi
-      -- rw[← List.getElem_append_right' a b'] Why?
-      have : (a ++ b')[a.length + i]'(by rw[List.length_append]; omega) = b'[i] := by
-        rw[List.getElem_append_right']
-        simp only [add_tsub_cancel_left]
-        omega
-      rw[← this]
-      apply habzero (a.length + i)
-      omega
-    have har: a = List.replicate a.length (fun _ => 0) := by
-      apply List.ext_getElem
-      . simp
-      . intro n_1 h₁ h₂
-        simp only [List.getElem_replicate]
-        exact hazero n_1 h₁
-    have hbr: b' = List.replicate b'.length (fun _ => 0) := by
-      apply List.ext_getElem
-      . simp
-      . intro n_1 h₁ h₂
-        simp only [List.getElem_replicate]
-        exact hbzero n_1 h₁
-    have habk : a.length + b'.length < k := by omega
-    have hk : (List.replicate k (fun _ => 0)) = (List.replicate (a.length + b'.length) (fun _ => 0)) ++ (List.replicate (k - a.length - b'.length) (fun _ : Fin n => (0 : Fin (b + 2)))) := by
-      simp[List.append_replicate_replicate]
-      omega
-    have hcx : c = padZeroes (k - a.length - b'.length) x := by
-      rw[har, hbr] at hkxabc
-      rw[List.append_assoc, ← padZeroes, ← padZeroes, padZeroes_add] at hkxabc
-      simp only [padZeroes] at hkxabc
-      have : c = padZeroes (k - (a.length + b'.length)) x := by
-        apply List.eq_diff_of_replicate_append_eq
-        . exact hkxabc.symm
-        . omega
-      rw[this]
-      convert rfl using 2
-      omega
-    have hac : a ++ c = padZeroes (k - b'.length) x := by
-      rw[hcx, har]
-      simp only [padZeroes, List.length_replicate]
-      rw[← List.append_assoc]
-      simp only [List.length_replicate, List.append_replicate_replicate,
-        List.append_cancel_right_eq, List.replicate_inj, AddLeftCancelMonoid.add_eq_zero,
-        List.length_eq_zero, or_true, and_true]
-      omega
+-- theorem project_transStep [DecidableEq state](dfa : DFA (Fin (n + 1) → Fin (b+2)) state) (m : Fin (n + 1)) (x : Fin (b+2)) (f : (Fin n → Fin (b+2))) (p q : state) : dfa.transFrom [(recover_value m x f)] p = q → q ∈ ((project m dfa).transFrom [f] ⟨[p], by exact List.nodup_singleton p⟩).val := by
+--   simp only [DFAO.transFrom, NFA.transFrom, NFA.transList, project, List.bind_cons, List.bind_nil,
+--     List.append_nil, List.dedup_idem, List.mem_dedup, List.mem_map, FinEnum.mem_toList, true_and]
+--   intro a
+--   subst a
+--   simp_all only [exists_apply_eq_apply]
 
-    by_cases hkb : k - b'.length ≤ Fintype.card state
-    . have : Fintype.card state = (Fintype.card state - (k - b'.length)) + (k - b'.length) := by omega
-      rw[this, ← padZeroes_add (Fintype.card state - (k - b'.length)) (k - b'.length) x, ← hac]
-      apply h (a ++ c)
-      . exact haco
-    . simp only [not_le] at hkb
-      have hblen : 0 < b'.length := by
-        exact List.length_pos_of_ne_nil hne
-
-      specialize ih (k - b'.length - Fintype.card state) (by omega) (k - b'.length)
-      apply ih
-      . rw[← hac]
-        exact haco
-      . exact hkb
-      . rfl
-
-theorem DFA.bounded_accept [Fintype state] (dfa : DFA (Fin n → Fin (b+2)) state) (x : List (Fin n → Fin (b+2)))(h: dfa.acceptZero): ∀ z, (∃ k, z = padZeroes k x) ∧ dfa.eval z → dfa.eval (padZeroes (Fintype.card state) x) := by
-  have := DFAO.bounded_out dfa x true
-  intro z a
-  simp_all only [implies_true, true_implies, DFA.acceptZero]
-  obtain ⟨left, right⟩ := a
-  obtain ⟨w, h_1⟩ := left
-  subst h_1
-  apply this
-  · exact right
-
-theorem NFA.bounded_accept [Fintype state] [DecidableEq state] (nfa : NFA (Fin n → Fin (b+2)) state) (x : List (Fin n → Fin (b+2)))(h: nfa.acceptZero): ∀ z, (∃ k, z = padZeroes k x) ∧ nfa.eval z → nfa.eval (padZeroes (Fintype.card (ListND state)) x) := by
-  simp only [NFA.acceptZero, ← NFA.toDFA_eval] at *
-  have := DFA.bounded_accept (nfa.toDFA) x h
-  intro z a
-  simp_all only [and_imp, forall_exists_index]
-  obtain ⟨left, right⟩ := a
-  obtain ⟨w, h_1⟩ := left
-  subst h_1
-  apply this
-  · rfl
-  · exact right
-
-theorem project_correct [Fintype state] [DecidableEq state] (l : List ℕ) (m : Fin (l.length + 1)) (dfa : DFA (Fin (l.length +1) → Fin (b+2)) state) (h: dfa.acceptZero):
-  ∃ (x : ℕ), dfa.eval (inputToBase (b+2) (by norm_num) (l.insertNth m x) (by sorry)) ↔ (project m dfa).eval (padZeroes (Fintype.card (ListND state)) (inputToBase (b+2) (by omega) l (by sorry))):= by
-  sorry
+-- theorem project_transStep [DecidableEq state](dfa : DFA (Fin (n + 1) → Fin (b+2)) state) (m : Fin (n + 1)) (f : (Fin (n+1) → Fin (b+2))) (p q : state) : dfa.transFrom [f] p = q → q ∈ ((project m dfa).transFrom [remove_index m f] ⟨[p], by exact List.nodup_singleton p⟩).val := by
+--   simp only [DFAO.transFrom, NFA.transFrom, NFA.transList, project, List.bind_cons, List.bind_nil,
+--     List.append_nil, List.dedup_idem, List.mem_dedup, List.mem_map, FinEnum.mem_toList, true_and]
+--   intro h
+--   use f m
+--   simp[recover_value, insert_remove]
+--   exact h
