Automata/LeadingZeros.lean
@@ -1,0 +1,240 @@
+import Mathlib.Tactic
+import Automata.DFA
+import Automata.NFA
+import Automata.Boolean
+import Automata.Input
+import Automata.Replicate
+import Automata.Pumping
+import Automata.Equality
+
+def padZeroes (m : ℕ) (x : List (Fin n → Fin (b+2))) : List (Fin n → Fin (b+2)) :=
+  List.replicate m (fun _ => 0) ++ x
+
+theorem padZeroes_add (a b : ℕ) (x : List (Fin n → Fin (k+2))) : padZeroes a (padZeroes b x) = padZeroes (a + b) x := by
+  simp only [padZeroes]
+  rw[← List.append_assoc, List.replicate_append_add]
+
+theorem padZeroes_length (m : ℕ) (x : List (Fin n → Fin (b+2))) : (padZeroes m x).length = m + x.length := by
+  simp only [padZeroes]
+  rw[List.replicate_append_length]
+
+theorem padZeroes_zero (m i: ℕ) (x : List (Fin n → Fin (b+2))) (h : i < m) : (padZeroes m x)[i]'(by simp only [padZeroes, List.length_append, List.length_replicate]; omega) = fun _ => 0 := by
+  simp only [padZeroes]
+  rwa[List.getElem_of_replicate_append_left]
+
+theorem padZeroes_diff (a b: ℕ) (x y : List (Fin n → Fin (k+2))) (hab : a ≤ b) (h: (padZeroes a x) = (padZeroes b y)) : x = padZeroes (b - a) y := by
+  simp only [padZeroes] at *
+  apply List.eq_diff_of_replicate_append_eq
+  . exact h
+  . exact hab
+
+def DFA.respectZero (dfa : DFA (Fin n → Fin (b+2)) state) : Prop := ∀ (x : List (Fin n → Fin (b+2))), ∀ m, dfa.eval x ↔ dfa.eval (padZeroes m x)
+
+def NFA.respectZero [DecidableEq state] (nfa : NFA (Fin n → Fin (b+2)) state) : Prop := ∀ (x : List (Fin n → Fin (b+2))), ∀ m, nfa.eval x ↔ nfa.eval (padZeroes m x)
+
+theorem equality_respectZero : (eqBase (b + 2) l m n).respectZero := by
+  rw[DFA.respectZero]
+  intro x c
+  constructor
+  intro h
+  rw[padZeroes]
+  rw[DFAO.eval, DFAO.evalFrom, DFAO.transFrom_of_append]
+  nth_rw 1 [eqBase]
+  simp only [Fin.isValue, beq_iff_eq]
+  suffices: (DFAO.transFrom (eqBase (b + 2) l m n) (List.replicate c fun _ ↦ 0) (eqBase (b + 2) l m n).start) = 0
+  . rw[this]
+    simp[DFAO.eval, DFAO.evalFrom] at h
+    nth_rw 1 3 [eqBase] at h
+    simp only [Fin.isValue, beq_iff_eq] at h
+    exact h
+  nth_rw 2 [eqBase]
+  simp only [Fin.isValue]
+  apply eqBase_transFrom_zero 0 (List.replicate c fun _ ↦ 0) |>.mpr
+  constructor
+  . rfl
+  . intro f a
+    simp_all only [List.mem_replicate, ne_eq, Fin.val_zero]
+  . intro h
+    contrapose h; simp_all only [Bool.not_eq_true]
+    rw[padZeroes]
+    rw[DFAO.eval, DFAO.evalFrom, DFAO.transFrom_of_append]
+    nth_rw 1 [eqBase]
+    simp only [Fin.isValue, beq_iff_eq]
+    suffices: (DFAO.transFrom (eqBase (b + 2) l m n) (List.replicate c fun _ ↦ 0) (eqBase (b + 2) l m n).start) = 0
+    . rw[this]
+      simp[DFAO.eval, DFAO.evalFrom] at h
+      nth_rw 1 3 [eqBase] at h
+      simp only [Fin.isValue, beq_iff_eq] at h
+      exact h
+    nth_rw 2 [eqBase]
+    simp only [Fin.isValue]
+    apply eqBase_transFrom_zero 0 (List.replicate c fun _ ↦ 0) |>.mpr
+    simp_all only [Fin.isValue, List.mem_replicate, ne_eq, Fin.val_zero, and_imp, implies_true, and_self]
+
+def DFA.acceptZero (dfa : DFA (Fin n → Fin (b+2)) state) : Prop := ∀ (x : List (Fin n → Fin (b+2))), (dfa.eval x → ∀ m, dfa.eval (padZeroes m x))
+
+def NFA.acceptZero [DecidableEq state] (nfa : NFA (Fin n → Fin (b+2)) state) : Prop := ∀ (x : List (Fin n → Fin (b+2))), (nfa.eval x → ∀ m, nfa.eval (padZeroes m x))
+
+theorem DFA.acceptZero_of_respectZero (dfa : DFA (Fin n → Fin (b+2)) state) (h: dfa.respectZero) : dfa.acceptZero := by
+  rw[DFA.acceptZero]
+  rw[DFA.respectZero] at h
+  intro x hxo m
+  specialize h x m
+  exact h.mp hxo
+
+theorem NFA.acceptZero_of_respectZero [DecidableEq state] (nfa : NFA (Fin n → Fin (b+2)) state) (h: nfa.respectZero) : nfa.acceptZero := by
+  rw[NFA.acceptZero]
+  rw[NFA.respectZero] at h
+  intro x hxo m
+  specialize h x m
+  exact h.mp hxo
+
+-- Bounded acceptance theorems: If a DFA/NFA accepts some representation of a input, then there is a bound on the number of leading zeros needed for acceptance
+theorem DFAO.bounded_out [Fintype state] (dfao : DFAO (Fin n → Fin (b+2)) state out) (x : List (Fin n → Fin (b+2))) (o: out)(h: ∀ (x : List (Fin n → Fin (b+2))), dfao.eval x = o → (∀ m, dfao.eval (padZeroes m x) = o)) : ∀ k, dfao.eval (padZeroes k x) = o → dfao.eval (padZeroes (Fintype.card state) x) = o := by
+  rintro k hkxo
+  by_cases hkstate : k ≤ Fintype.card state
+  . have: Fintype.card state = (Fintype.card state - k) + k := by omega
+    rw[this, ← padZeroes_add (Fintype.card state - k) k x]
+    apply h
+    exact hkxo
+
+  simp only [not_le] at hkstate
+  -- Question: How to get this kind of descent argument work in lean?
+  . induction' hk : k - Fintype.card state using Nat.strong_induction_on  with d ih generalizing k
+    have hkxlen : Fintype.card state ≤ (padZeroes k x).length := by
+      simp only [padZeroes_length]
+      omega
+
+    obtain ⟨a, b', c, hkxabc, hablen, hne, hy⟩ := dfao.pumping_lemma_eval hkxo hkxlen
+    have haco : dfao.eval (a ++ c) = o := by
+      apply hy
+      simp only [Language.mem_mul, exists_exists_and_exists_and_eq_and, List.append_assoc]
+      use a, (by exact rfl), [], (by exact Language.nil_mem_kstar {b'}), c, (by exact rfl)
+      simp only [List.nil_append]
+    -- have hblen : 0 < b'.length := by
+    --   exact List.length_pos_of_ne_nil hne
+
+    have habzero : ∀ i, ∀ (hi: i < a.length + b'.length),  (a ++ b')[i]' (by rw[List.length_append]; exact hi) = fun _ => 0 := by
+      intro i hi
+      rw[← List.getElem_append_left (a++b') c]
+      trans (padZeroes k x)[i]
+      congr 1
+      . exact hkxabc.symm
+      . apply padZeroes_zero k
+        omega
+      simp only [List.append_assoc, List.length_append]
+      . omega
+
+    have hazero : ∀ i, ∀ (hi: i < a.length),  a[i]' (by omega) = fun _ => 0 := by
+      intro i hi
+      rw[← List.getElem_append_left a b']
+      apply habzero i
+      . omega
+    have hbzero : ∀ i, ∀ (hi: i < b'.length),  b'[i]' (by omega) = fun _ => 0 := by
+      intro i hi
+      -- rw[← List.getElem_append_right' a b'] Why?
+      have : (a ++ b')[a.length + i]'(by rw[List.length_append]; omega) = b'[i] := by
+        rw[List.getElem_append_right']
+        simp only [add_tsub_cancel_left]
+        omega
+      rw[← this]
+      apply habzero (a.length + i)
+      omega
+    have har: a = List.replicate a.length (fun _ => 0) := by
+      apply List.ext_getElem
+      . simp
+      . intro n_1 h₁ h₂
+        simp only [List.getElem_replicate]
+        exact hazero n_1 h₁
+    have hbr: b' = List.replicate b'.length (fun _ => 0) := by
+      apply List.ext_getElem
+      . simp
+      . intro n_1 h₁ h₂
+        simp only [List.getElem_replicate]
+        exact hbzero n_1 h₁
+    have habk : a.length + b'.length < k := by omega
+    have hk : (List.replicate k (fun _ => 0)) = (List.replicate (a.length + b'.length) (fun _ => 0)) ++ (List.replicate (k - a.length - b'.length) (fun _ : Fin n => (0 : Fin (b + 2)))) := by
+      simp[List.append_replicate_replicate]
+      omega
+    have hcx : c = padZeroes (k - a.length - b'.length) x := by
+      rw[har, hbr] at hkxabc
+      rw[List.append_assoc, ← padZeroes, ← padZeroes, padZeroes_add] at hkxabc
+      simp only [padZeroes] at hkxabc
+      have : c = padZeroes (k - (a.length + b'.length)) x := by
+        apply List.eq_diff_of_replicate_append_eq
+        . exact hkxabc.symm
+        . omega
+      rw[this]
+      convert rfl using 2
+      omega
+    have hac : a ++ c = padZeroes (k - b'.length) x := by
+      rw[hcx, har]
+      simp only [padZeroes, List.length_replicate]
+      rw[← List.append_assoc]
+      simp only [List.length_replicate, List.append_replicate_replicate,
+        List.append_cancel_right_eq, List.replicate_inj, AddLeftCancelMonoid.add_eq_zero,
+        List.length_eq_zero, or_true, and_true]
+      omega
+
+    by_cases hkb : k - b'.length ≤ Fintype.card state
+    . have : Fintype.card state = (Fintype.card state - (k - b'.length)) + (k - b'.length) := by omega
+      rw[this, ← padZeroes_add (Fintype.card state - (k - b'.length)) (k - b'.length) x, ← hac]
+      apply h (a ++ c)
+      . exact haco
+    . simp only [not_le] at hkb
+      have hblen : 0 < b'.length := by
+        exact List.length_pos_of_ne_nil hne
+
+      specialize ih (k - b'.length - Fintype.card state) (by omega) (k - b'.length)
+      apply ih
+      . rw[← hac]
+        exact haco
+      . exact hkb
+      . rfl
+
+theorem DFA.bounded_accept [Fintype state] (dfa : DFA (Fin n → Fin (b+2)) state) (x : List (Fin n → Fin (b+2)))(h: dfa.acceptZero): ∀ z, (∃ k, z = padZeroes k x) ∧ dfa.eval z → dfa.eval (padZeroes (Fintype.card state) x) := by
+  have := DFAO.bounded_out dfa x true
+  intro z a
+  simp_all only [implies_true, true_implies, DFA.acceptZero]
+  obtain ⟨left, right⟩ := a
+  obtain ⟨w, h_1⟩ := left
+  subst h_1
+  apply this
+  · exact right
+
+theorem NFA.bounded_accept [Fintype state] [DecidableEq state] (nfa : NFA (Fin n → Fin (b+2)) state) (x : List (Fin n → Fin (b+2)))(h: nfa.acceptZero): ∀ z, (∃ k, z = padZeroes k x) ∧ nfa.eval z → nfa.eval (padZeroes (Fintype.card (ListND state)) x) := by
+  simp only [NFA.acceptZero, ← NFA.toDFA_eval] at *
+  have := DFA.bounded_accept (nfa.toDFA) x h
+  intro z a
+  simp_all only [and_imp, forall_exists_index]
+  obtain ⟨left, right⟩ := a
+  obtain ⟨w, h_1⟩ := left
+  subst h_1
+  apply this
+  · rfl
+  · exact right
+
+
+
+-- Legacy
+
+-- theorem equality_acceptZero : (eqBase (b + 2) l m n).acceptZero := by
+--   rw[DFA.acceptZero]
+--   intro x h c
+--   rw[padZeroes]
+--   rw[DFAO.eval, DFAO.evalFrom, DFAO.transFrom_of_append]
+--   nth_rw 1 [eqBase]
+--   simp only [Fin.isValue, beq_iff_eq]
+--   suffices: (DFAO.transFrom (eqBase (b + 2) l m n) (List.replicate c fun _ ↦ 0) (eqBase (b + 2) l m n).start) = 0
+--   . rw[this]
+--     simp[DFAO.eval, DFAO.evalFrom] at h
+--     nth_rw 1 3 [eqBase] at h
+--     simp only [Fin.isValue, beq_iff_eq] at h
+--     exact h
+--   nth_rw 2 [eqBase]
+--   simp only [Fin.isValue]
+--   apply eqBase_transFrom_zero 0 (List.replicate c fun _ ↦ 0) |>.mpr
+--   constructor
+--   . rfl
+--   . intro f a
+--     simp_all only [List.mem_replicate, ne_eq, Fin.val_zero]
